Started reworking the linear checker

theories/Linear.v
@@ -14,7 +14,7 @@ Import Utility.Maps.
 Open Scope Z_scope.
 Import ListNotations.
 
-Definition term_lower_bound (coef : Z) (var : string) (dom : Domain.Domain) : option Z :=
+Definition dom_term_lower_bound (coef : Z) (dom : Domain.Domain) : option Z :=
   if coef >? 0
   then match (Domain.d_lb dom) with
        | zz lb => Some (coef * lb)
@@ -25,25 +25,33 @@ Definition term_lower_bound (coef : Z) (var : string) (dom : Domain.Domain) : op
        | _ => None
        end.
 
-Fixpoint lower_bound (terms : list (Z * string)) (doms : Domains) :=
-  match terms with
-  | [] => Some 0
-  | (coef, v) :: tail =>
-      match smap.find v doms with
-      | Some dom => 
-          match term_lower_bound coef v dom, lower_bound tail doms with
-          | Some term_lb, Some tail_lb => Some (term_lb + tail_lb)
-          | _, _ => None
-          end
+Definition term_lower_bound (term : Z * Var) (doms : Domains) : option Z :=
+  match term with
+  | (coef, var_name ident) => match smap.find ident doms with
+      | Some dom => dom_term_lower_bound coef dom
       | None => None
       end
+  | (coef, const value) => Some (coef * value)
   end.
+
+Definition accumulate_terms (doms: Domains) (maybe_acc : option Z) (term : Z * Var) : option Z :=
+  match maybe_acc with
+  | Some accumulator =>
+    match term_lower_bound term doms with
+    | Some value => Some (accumulator + value)
+    | None => None
+    end
+  | None => None
+  end.
+
+Fixpoint compute_linear_lower_bound (terms : list (Z * Var)) (doms : Domains) : option Z := 
+  fold_left (accumulate_terms doms) terms (Some Z.zero).
 
 Definition linear_checker (fact : ProofFact) (c : LinearConstraint) :=
   match Deduction.infer_domains fact with
   (* Currently information on what variable is r.h.s. is not used. *)
   | Some (doms, _) => 
-    match lower_bound (c.(l_terms)) doms with
+    match compute_linear_lower_bound (c.(l_terms)) doms with
     | None => false
     | Some lb => lb >? c.(l_bound)
     end
@@ -51,19 +59,19 @@ Definition linear_checker (fact : ProofFact) (c : LinearConstraint) :=
   | None => false
   end.
 
-Lemma term_bound_validity : forall
-  (coef : Z) (var : string) (dom : Domain.Domain)
+Lemma dom_bound_validity : forall
+  (coef : Z) (dom : Domain.Domain)
   (val : Z)
   (bound : Z),
   Domain.is_in_dom val dom ->
-  term_lower_bound coef var dom = Some bound ->
+  dom_term_lower_bound coef dom = Some bound ->
   bound <= coef * val.
 Proof.
-  intros coef var dom sol bound Hvalid Elb.
+  intros coef dom sol bound Hvalid Elb.
   unfold Domain.is_in_dom in Hvalid.
   destruct dom; simpl in Hvalid.
   destruct Hvalid as [Hub [Hlb _]].
-  unfold term_lower_bound in Elb.
+  unfold dom_term_lower_bound in Elb.
   simpl in Elb.
   destruct (coef >? 0) eqn:Hsign.
   - destruct d_lb; zext_as_z; inversion Elb as [Elb'].
@@ -72,13 +80,22 @@ Proof.
     apply Z.mul_le_mono_nonpos_l ; lia.
 Qed.
 
-Lemma bound_validity : forall
-  (terms : list (Z * string)) (doms : Domains)
-  (sol : string -> Z)
-  (bound : Z),
-  sol_in_doms sol doms -> lower_bound terms doms = Some bound ->
-  bound <= evaluate_linear terms sol.
+Lemma term_bound_validity : forall
+  (term : Z * Var) (doms : Domains) (sol : Assignment) (bound : Z),
+  sol_in_doms sol doms ->
+  term_lower_bound term doms = Some bound ->
+  bound <= evaluate_term sol term.
 Proof.
+Admitted.
+
+Lemma bound_validity : forall
+  (terms : list (Z * Var)) (doms : Domains)
+  (sol : Assignment)
+  (bound : Z),
+  sol_in_doms sol doms -> compute_linear_lower_bound terms doms = Some bound ->
+  bound <= evaluate_linear sol terms.
+Proof.
+  (*  
   intros terms doms sol bound Hvalid.
   generalize dependent bound.
   Opaque term_lower_bound.
@@ -100,10 +117,12 @@ Proof.
     reflexivity.
   }
   lia.
-Qed.
+     Qed.*)
+
+Admitted.
 
 Theorem linear_checker_soundness : forall
-  (fact : ProofFact) (sol : string -> Z) (c : LinearConstraint),
+  (fact : ProofFact) (sol : Assignment) (c : LinearConstraint),
   Linear c sol ->
   Is_true (linear_checker fact c)
   -> fact_valid sol fact.
@@ -116,9 +135,9 @@ Proof.
   intros Hsat Hbound.
   destruct (infer_domains fact) as [[doms rhs_var]|] eqn:Edoms ; try contradiction.
   apply infer_domains_correct with (doms := doms) (xconsq := rhs_var) ; try apply Edoms.
-  destruct (lower_bound lin_terms doms) as [lb|] eqn:Elb ; try contradiction.
+  destruct (compute_linear_lower_bound lin_terms doms) as [lb|] eqn:Elb ; try contradiction.
   apply Is_true_eq_true, Z.gtb_gt, Z.gt_lt in Hbound.
   intros Hvalid.
-  enough (lb <= evaluate_linear lin_terms sol) by lia.
+  enough (lb <= evaluate_linear sol lin_terms) by lia.
   apply bound_validity with (doms := doms) ; assumption.
 Qed.
